proof/crypto_stream/chacha20/ref/ChaCha20_sref_proof.ec
@@ -4,55 +4,277 @@ require import ChaCha20_Spec ChaCha20_pref ChaCha20_pref_proof ChaCha20_sref.
 require import Array3 Array8 Array16.
 require import WArray64.
 
-equiv init : ChaCha20_pref.M.init ~ ChaCha20_sref.M.init :
-  ={key, nonce, counter, Glob.mem} ==>
+(* ------------------------------------------------------------------------------- *)
+(* We start by cloning ChaCha20_sref but using "int" instead of W64.t for pointer. *)
+(* Compare to ChaCha20_pref we change the way of writting into memory              *)
+theory ChaCha20_srefi.
+
+module M = {
+  include ChaCha20_pref.M [init, line, quarter_round, column_round, diagonal_round, round, rounds, sum_states, update_ptr, increment_counter]
+
+  proc store (output plain:address, len: int, k:W32.t Array16.t) : int * int * int = {
+    var i:int;
+    
+    i <- 0;
+    while ((i < 16)) {
+      Glob.mem <- storeW32 Glob.mem (output + 4 * i) (k.[i] `^` loadW32 Glob.mem (plain + 4 * i));
+      i <- (i + 1);
+    }
+    (output, plain, len) <@ update_ptr (output, plain, len, 64);
+    return (output, plain, len);
+  }
+
+  proc store_last (output plain:address, len: int, k:W32.t Array16.t) = {
+    var j:int;
+    j <- 0;
+    while (j < len) {
+      Glob.mem <- storeW8 Glob.mem (output + j) 
+       (loadW8 Glob.mem (plain + j) `^` (get8 (WArray64.init32 (fun i => k.[i])) j));
+      j <- j + 1;
+    }
+  }
+
+  proc chacha20_ref (output plain:address, len:int, key nonce: address, counter:W32.t) : unit = {
+    
+    var st:W32.t Array16.t;
+    var k:W32.t Array16.t;
+
+    st <@ init (key, nonce, counter);    
+    while (64 <= len) {
+      k <@ rounds (st);
+      k <@ sum_states (k, st);
+      (output, plain, len) <@ store (output, plain, len, k);
+      st <@ increment_counter (st);
+    }
+    if (0 < len) {
+      k <@ rounds (st);
+      k <@ sum_states (k, st);
+      store_last (output, plain, len, k);
+    }
+  }   
+}.
+
+end ChaCha20_srefi.
+
+lemma get_storesE m p l j: (stores m p l).[j] = if p <= j < p + size l then nth W8.zero l (j - p) else m.[j].
+proof.
+  elim: l m p => [ | w l hrec] m p.
+  + by rewrite /stores /= /#.
+  rewrite stores_cons hrec /= get_setE.  smt (size_ge0).
+qed.
+  
+lemma get_storeW32E m p (w:W32.t) j :
+  (storeW32 m p w).[j] = if p <= j < p + 4 then w \bits8 (j - p) else m.[j].
+proof. rewrite storeW32E /= get_storesE /= /#. qed.
+
+phoare store_pref_spec output0 plain0 len0 k0 mem0 : [ChaCha20_pref.M.store : 
+  output = output0 /\ plain = plain0 /\ len = len0 /\ k = k0 /\ Glob.mem = mem0 /\ 
+  0 <= len /\ inv_ptr output plain len 
+  ==>
+  inv_ptr res.`1 res.`2 res.`3 /\ res = (output0 + min 64 len0, plain0 + min 64 len0, len0 - min 64 len0) /\
+  forall j, 
+    Glob.mem.[j] =
+      if in_range output0 (min 64 len0) j then
+        let j = j - output0 in
+        (init32 (fun (i0 : int) => k0.[i0])).[j] `^` mem0.[plain0 + j]
+      else mem0.[j]]= 1%r.
+proof.
+  proc; inline *; wp.
+  while (0 <= i <= min 64 len /\ 
+    forall j, Glob.mem.[j] = if in_range output i j then k8.[j - output] else mem0.[j]) (min 64 len - i).
+  + move=> z;wp; skip => /> &hr h0i _ hj hi; split; 2: smt().
+    split; 1: smt().
+    by move=> j; rewrite storeW8E get_setE hj; smt().
+  wp; while(0 <= i <= min 64 len /\
+    forall j, 0 <= j < i => k8.[j] = k8_0.[j] `^` loadW8 Glob.mem (plain + j)) (min 64 len - i).
+  + move=> z;wp; skip => />; smt (WArray64.get_setE).
+  by wp; skip => /> /#.
+qed.
+
+phoare store_srefi_spec output0 plain0 len0 k0 mem0 : [ChaCha20_srefi.M.store : 
+  output = output0 /\ plain = plain0 /\ len = len0 /\ k = k0 /\ Glob.mem = mem0 /\ 
+  64 <= len /\ inv_ptr output plain len 
+  ==>
+  res = (output0 + 64, plain0 + 64, len0 - 64) /\ 
+  forall j, 
+    Glob.mem.[j] =
+      if in_range output0 64 j then
+        let j = j - output0 in
+        (init32 (fun (i0 : int) => k0.[i0])).[j] `^` mem0.[plain0 + j]
+      else mem0.[j]]= 1%r.
+proof.
+  proc; inline *; wp.
+  while (0 <= i <= 16 /\ inv_ptr output plain 64 /\ 
+    forall j, 
+      Glob.mem.[j] = 
+      if in_range output (4 * i) j then 
+        let j = j - output in
+        (init32 (fun (i0 : int) => k.[i0])).[j] `^` mem0.[plain + j]
+      else mem0.[j]) (16 - i).
+  + move=> z;wp; skip=> /> &hr _ hi16 hinv hj h0i; split; 2: smt().
+    split; 1: smt().
+    move=> j. rewrite get_storeW32E.
+    have hhi: 0 <= 4 * i{hr} /\ 4 * i{hr} + 4 <= 64 by smt(). 
+    case: (output{hr} + 4 * i{hr} <= j < output{hr} + 4 * i{hr} + 4)=> [ h1 | /#].
+    rewrite (_: in_range output{hr} (4 * (i{hr} +1)) j) 1:/# /=. 
+    rewrite xorb8E 1:/# /init32 WArray64.initE /= (_:0 <= j - output{hr} < 64) 1:/# /=.
+    rewrite loadW32_bits8 1:/# /loadW8 hj.
+    rewrite (_: !in_range output{hr} (4 * i{hr}) (plain{hr} + 4 * i{hr} + (j - (output{hr} + 4 * i{hr})))) 1:/#.
+    by have [h2 h3] /# := euclideUl 4 i{hr} ((j - output{hr}) - 4*i{hr}) (j-output{hr}) _ _;
+        [rewrite -divz_eq; ring |  smt()].
+  wp; skip => /> &hr hlen hinv;split; 1:smt().
+  move=> mem i0; split; 1: smt().
+  move=> ???; have ->> /= : i0 = 16; smt().
+qed.
+
+phoare store_last_srefi_spec output0 plain0 len0 k0 mem0 : [ChaCha20_srefi.M.store_last : 
+  output = output0 /\ plain = plain0 /\ len = len0 /\ k = k0 /\ Glob.mem = mem0 /\ 
+  0 <= len < 64 /\ inv_ptr output plain len 
+  ==>
+  forall j, 
+    Glob.mem.[j] =
+      if in_range output0 len0 j then
+        let j = j - output0 in
+        (init32 (fun (i0 : int) => k0.[i0])).[j] `^` mem0.[plain0 + j]
+      else mem0.[j]]= 1%r.
+proof.
+  proc; inline *; wp.
+  while (0 <= j <= len /\ inv_ptr output plain len /\ 
+    forall i, 
+      Glob.mem.[i] = 
+      if in_range output j i then 
+        let i = i - output in
+        (init32 (fun (i0 : int) => k.[i0])).[i] `^` mem0.[plain + i]
+      else mem0.[i]) (len - j).
+  + move=> z;wp; skip=> /> &hr _ hi16 hinv hj h0i; split; 2: smt().
+    split; 1: smt().
+    move=> i. 
+    rewrite storeW8E get_setE W8.xorwC /get8 /loadW8.
+    case: (i = output{hr} + j{hr}) => [-> | hne]. smt().
+    rewrite hj.
+    have -> // : in_range output{hr} j{hr} i = in_range output{hr} (j{hr} + 1) i. smt().
+  wp; skip => /> &hr h0len hlen hinv;split; 1: smt().
+  move=> mem j0; split; 1: smt().
+  move=> ???; have ->> /= : j0 = len{hr}; smt().
+qed.
+
+(* FIXME: move this *)
+axiom mem_eq_ext (m1 m2:global_mem_t) : (forall j, m1.[j] = m2.[j]) => m1 = m2.
+
+equiv eq_store32_pref_srefi len0 : ChaCha20_pref.M.store ~ ChaCha20_srefi.M.store :
+  ={output, plain, len, k, Glob.mem} /\ len{1} = len0 /\ (inv_ptr output plain len){1} /\ 64 <= len{1} ==> 
+  ={res, Glob.mem} /\ res{1}.`3 = len0 - 64 /\ (inv_ptr res.`1 res.`2 res.`3){1}.
+proof.
+  proc *.
+  ecall{1}(store_pref_spec output{1} plain{1} len{1} k{1} Glob.mem{1}).
+  ecall{2}(store_srefi_spec output{1} plain{1} len{1} k{1} Glob.mem{1}).
+  skip => /> &1 &2 4!<- /= h hlen. rewrite h hlen /= => m2 hm2.
+  have -> : min 64 len{1} = 64 by smt().
+  rewrite  /= (_: 0 <= len{1}) 1:/# /= => m1 hinv hm1.
+  by apply mem_eq_ext => j;rewrite hm1 hm2.
+qed.
+
+equiv eq_store_last_pref_srefi : ChaCha20_pref.M.store ~ ChaCha20_srefi.M.store_last :
+  ={output, plain, len, k, Glob.mem} /\ (inv_ptr output plain len){1} /\ 0 <= len{1} < 64 ==> 
+  ={Glob.mem}.
+proof.
+  proc *.
+  ecall{1}(store_pref_spec output{1} plain{1} len{1} k{1} Glob.mem{1}).
+  ecall{2}(store_last_srefi_spec output{1} plain{1} len{1} k{1} Glob.mem{1}).
+  skip => /> &1 &2 4!<- /= h h0len hlen; rewrite h h0len hlen /= => m2 hm2 m1 _ hm1.
+  by apply mem_eq_ext => j;rewrite hm1 hm2 /#.
+qed.
+
+equiv eq_chacha20_pref_srefi : ChaCha20_pref.M.chacha20_ref ~ ChaCha20_srefi.M.chacha20_ref : 
+   ={output, plain, len, key, nonce, counter, Glob.mem} /\ (inv_ptr output plain len){1} ==>
+   ={Glob.mem}.
+proof.
+  proc => /=.
+  splitwhile{1} 2 : (64 <= len).
+  seq 2 2 : (={st, output, plain, len, Glob.mem} /\ (inv_ptr output plain len){1} /\ len{1} < 64).
+  + while (={st, output, plain, len, Glob.mem} /\ (inv_ptr output plain len){1}).
+    + call (_:true); 1: sim.
+      ecall (eq_store32_pref_srefi len{1}) => /=.
+      conseq (_: ={k,st}); 1: by move=> /> /#.
+      by sim.
+    conseq (_: ={st}); 1: by move=> /> /#.
+    by sim.  
+  if{2}; last by rcondf{1} 1; auto.
+  rcondt{1} 1; 1: by auto.
+  rcondf{1} 5.
+  + move=> &m2. 
+    swap -1; inline ChaCha20_pref.M.store ChaCha20_pref.M.update_ptr; wp.
+    swap 6 -5; sp.  
+    while (i <= min 64 len0); 1: by wp;skip => /#.
+    by wp; conseq (_: true) => //; smt().
+  call{1} (_:true ==> true); 1:islossless.
+  call eq_store_last_pref_srefi => /=.
+  conseq (_: ={output, plain, len, k, Glob.mem}); 1:smt().
+  by sim.
+qed.
+
+(* ------------------------------------------------------------------------------- *)
+(* We now prove that ChaCha20_srefi, is equivalent to the concret implementation   *)
+(* ChaCha20_sref                                                                   *)
+
+op good_ptr (output plain len : int) =  
+  output + len < W64.modulus /\
+  plain + len < W64.modulus.
+
+equiv eq_init_srefi_sref : ChaCha20_srefi.M.init ~ ChaCha20_sref.M.init :
+  key{1} = to_uint key{2} /\ nonce{1} = to_uint nonce{2} /\  (key + 32 < W64.modulus /\ nonce + 12 < W64.modulus){1} /\
+    ={Glob.mem, counter} 
+  ==>
   ={res}.
 proof.
   proc.
-  while (={i,st, nonce, Glob.mem} /\ 0 <= i{1}).
-  + wp; skip => /> &2 2?.
-    by rewrite Array3.get_setE //= /#. 
-  wp;while(={i,st,key, Glob.mem} /\ 0 <= i{1}).
-  + wp;skip => /> &1 ??.
-    by rewrite Array8.get_setE //= /#.
+  while (={i,st, Glob.mem} /\ nonce{1} = to_uint nonce{2} /\ (nonce + 12 < W64.modulus /\ 0 <= i){1}).
+  + wp; skip => /> &2 3?.
+    have heq : to_uint (W64.of_int (4 * i{2})) = 4 * i{2}.
+    + by rewrite to_uint_small /= /#. 
+    by rewrite Array3.get_setE //= to_uintD_small heq /= /#. 
+  wp;while(={i,st, Glob.mem} /\ key{1} = to_uint key{2} /\ (key + 32 < W64.modulus /\ 0 <= i){1}).
+  + wp;skip => /> &2 3?.
+    have heq : to_uint (W64.of_int (4 * i{2})) = 4 * i{2}.
+    + by rewrite to_uint_small /= /#.
+    by rewrite Array8.get_setE //= to_uintD_small heq /= /#.
   wp;skip => />.
 qed.
 
-equiv copy_state : ChaCha20_pref.M.copy_state ~ ChaCha20_sref.M.copy_state :
-  ={st} ==> res{1} = res{2}.`1.[15 <- res{2}.`2].
+phoare copy_state_sref_spec st0 : [ChaCha20_sref.M.copy_state : st0 = st ==> st0 = res.`1.[15 <- res.`2]] = 1%r. 
 proof.
-  proc => /=.
-  conseq (_: Array16.all_eq k{1} k{2}.[15 <- s_k15{2}]). 
-  + by move=> *;apply Array16.all_eq_eq.
-  by unroll for {2} 5; wp; skip => />.
+  proc.
+  conseq (_: Array16.all_eq st0 k.[15 <- s_k15]). 
+  + by move=> ? -> /= ??; rewrite Array16.ext_eq_all.
+  by unroll for ^while; wp; skip => />.
 qed.
 
-equiv line_spec i ki: ChaCha20_pref.M.line ~ ChaCha20_sref.M.line : 
-    (0 <= i < 16 /\ ={a,b,c,r} /\ k{1} = k{2}.[i <- ki] /\ (a <> i /\ b <> i /\ c <> i){1}) ==>
+equiv line_spec i ki: ChaCha20_srefi.M.line ~ ChaCha20_sref.M.line : 
+    (0 <= i < 16 /\ ={a,b,c,r} /\ k{1} = k{2}.[i <- ki] /\ (a <> i /\ b <> i /\ c <> i /\ 0 <=r < 256){1}) ==>
     res{1} = res{2}.[i <- ki].
 proof.
-  proc;wp;skip => /> &2 h0i hi ha hb hc.
+  proc;wp;skip => /> &2 h0i hi ha hb hc h0r hr2_8.
   rewrite !(Array16.get_setE _ i) // ha hb /=.
   rewrite (Array16.set_set_if _ i) (eq_sym i) ha /=.
   rewrite (Array16.set_set_if _ i) (eq_sym i) hc /=.
   congr; congr.
   rewrite (Array16.set_set_if _ i) (eq_sym i) hc /=.
-  by rewrite !(Array16.get_setE _ i) // hc ha.
+  rewrite x86_ROL_32_E /= !(Array16.get_setE _ i) // hc ha /= modz_small //.
 qed.
 
-equiv quarter_round_spec i ki: ChaCha20_pref.M.quarter_round ~ ChaCha20_sref.M.quarter_round : 
+equiv quarter_round_spec i ki: ChaCha20_srefi.M.quarter_round ~ ChaCha20_sref.M.quarter_round : 
     (0 <= i < 16 /\ ={a,b,c,d} /\ k{1} = k{2}.[i <- ki] /\ (a <> i /\ b <> i /\ c <> i /\ d<>i){1}) ==>
     res{1} = res{2}.[i <- ki].
 proof.
   proc; do 4! call (line_spec i ki);skip => />.
 qed.
 
-equiv rounds : ChaCha20_pref.M.rounds ~ ChaCha20_sref.M.rounds :
+equiv eq_rounds_srefi_sref : ChaCha20_srefi.M.rounds ~ ChaCha20_sref.M.rounds :
   k{1} = k{2}.[15 <- k15{2}] ==>
   res{1} = res{2}.`1.[15 <- res{2}.`2].
 proof.
   proc => /=.
-  while ( ={c} /\ k{1} = k{2}.[15 <- k15{2}]);last by wp;skip.
+  while ( c{1} = to_uint c{2} /\ 0 <= c{1} /\ k{1} = k{2}.[15 <- k15{2}]);last by wp;skip.
   inline{1} ChaCha20_pref.M.round ChaCha20_pref.M.column_round ChaCha20_pref.M.diagonal_round.
   wp. 
   ecall (quarter_round_spec 15 k15{2}) => /=.
@@ -65,220 +287,192 @@ proof.
   wp.
   ecall (quarter_round_spec 15 k15{2}) => /=.
   ecall (quarter_round_spec 15 k15{2}) => /=.
-  by wp;skip => /> *;split => *; rewrite Array16.set_set_if /= Array16.set_notmod.
+  wp;skip => /> *; split => *; rewrite Array16.set_set_if /= Array16.set_notmod //=.
+  rewrite ultE /=.
+  have -> /= /#: to_uint (c{2} + W32.one) = to_uint c{2} + 1.
+  by rewrite to_uintD_small //= /#.
 qed.
 
-equiv sum_states : ChaCha20_pref.M.sum_states ~ ChaCha20_sref.M.sum_states :
+equiv eq_sum_states_srefi_sref : ChaCha20_pref.M.sum_states ~ ChaCha20_sref.M.sum_states :
   ={st} /\ k{1} = k{2}.[15 <- k15{2}] ==>
   res{1} = res{2}.`1.[15 <- res{2}.`2].
 proof.
   proc => /=.  
-  unroll for{1} 2; unroll for{2} 2.
+  unroll for{1} ^while; unroll for{2} ^while.
   conseq (_: all_eq k{1} k{2}.[15 <- k15{2}]).
   + by move=> &1 &2 _ k1 k2 k15 /Array16.all_eq_eq. 
   wp; skip => />.
 qed.
 
-clone import ExactIter as Loop0 with
-   type t <- W64.t * W64.t * W32.t Array16.t,
-   op c <- 4,
-   op step <- 1
-   proof * by done.
-
-module Body = {
-  proc body (t: W64.t * W64.t * W32.t Array16.t, i:int) = {
-    var output, plain, k;
-    (output, plain, k) <- t;
-    Glob.mem <-                
-       storeW8 Glob.mem (output + (of_int i)%W64)       
-          (get8 ((init32 (fun (i0 : int) => k.[i0])))%WArray64 i `^` loadW8 Glob.mem (plain + (of_int i)%W64));
-    return t;
-  }
-}.
-
-lemma load_storeW8 m p1 p2 w: 
-  loadW8 (storeW8 m p1 w) p2 = if p2 = p1 then w else loadW8 m p2.
-proof. by rewrite /loadW8 storeW8E Jasmin_memory.get_setE. qed.
-
-equiv store_store32 len0 : ChaCha20_pref.M.store ~ ChaCha20_pref.M.store32 : 
-  ={Glob.mem, k, output, plain, len} /\ W32.of_int 64 \ule len{1} /\
-  (inv_ptr output plain (to_uint len)){1} /\ len{1} = len0
-  ==>
-  ={Glob.mem, res} /\ (inv_ptr res.`1 res.`2 (to_uint res.`3)){1} /\ res{1}.`3 = len0 - W32.of_int 64.
-proof.
-  proc.
-  inline ChaCha20_pref.M.update_ptr;wp => /=.
-  transitivity{1} { Loop(Body).loop1((output, plain, k), 64);}
-       (={Glob.mem, output, plain, len, k} /\ (of_int 64)%W32 \ule len{1} ==> ={Glob.mem, output, plain, len, k} /\ i{1} = 64)
-       (={Glob.mem, k, output, plain, len} /\
-         ((of_int 64)%W32 \ule len{1}) /\ inv_ptr output{1} plain{1} (to_uint len{1}) /\ len{1} = len0 ==>
-        ={Glob.mem, output, plain, len} /\ inv_ptr (output{1} + (of_int 64)%W64) (plain{1} + (of_int 64)%W64) (to_uint (len{1} - (of_int 64)%W32)) /\
-        len{1} = len0).
-  + by move=> /> &2 *;exists Glob.mem{2} k{2} len{2} output{2} plain{2}. 
-  + by move=> />.
-  + inline *.
-    while ( ={Glob.mem, output, plain, len, k} /\ i{1} = i0{2} /\ 0 <= i{1} <= 64 /\ (t = (output, plain, k)){2} /\ 64 <= to_uint len{1} /\ n0{2} = 64).
-    + by auto => /> &2 h1 h2 h3;rewrite !W32.ultE !W32.to_uint_small /= /#.
-    by auto => /> &2;rewrite W32.uleE W32.ultE /= /#.
-  transitivity{1} { Loop(Body).loopc((output, plain, k), 16);}
-       (={Glob.mem, output, plain, len, k} ==> ={Glob.mem, output, plain, len, k})
-       (={Glob.mem, k, output, plain, len} /\
-         ((of_int 64)%W32 \ule len{1}) /\ inv_ptr output{1} plain{1} (to_uint len{1}) /\ len{1} = len0 ==>
-        ={Glob.mem, output, plain, len} /\ inv_ptr (output{1} + (of_int 64)%W64) (plain{1} + (of_int 64)%W64) (to_uint (len{1} - (of_int 64)%W32)) /\
-        len{1} = len0).
-  + by move=> /> &2 *;exists Glob.mem{2} k{2} len{2} output{2} plain{2}. 
-  + by move=> />.
-  + by call (loop1_loopc Body); skip.
-  inline *;wp.
-  while ( ={Glob.mem, k, output, plain, len} /\ inv_ptr output{1} plain{1} (to_uint len{1}) /\ 64 <= to_uint len{1} /\
-          n0{1} = 16 /\ i0{1} = i{2} /\  0 <= i{2} /\ (t = (output, plain, k)){1}).
-  + unroll for {1} 2;wp;skip => |> &2 h1 h2 h3 h4. 
-    pose ini := WArray64.init32 (fun (i0 : int) => k{2}.[i0]).
-    split; 2: smt().
-    have b0 : 0 <= 4 * i{2} <= to_uint len{2} by smt().
-    have b1 : 0 <= 4 * i{2} + 1 <= to_uint len{2} by smt().
-    have b2 : 0 <= 4 * i{2} + 2 <= to_uint len{2} by smt().
-    have b3 : 0 <= 4 * i{2} + 3 <= to_uint len{2} by smt().
-    do 6!rewrite load_storeW8 (inv_ptr_disj (to_uint len{2})) // 1:-StdOrder.IntOrder.ltr_subl_addl 1:/# /=. 
-    rewrite -load4u8.
-    have -> : k{2}.[i{2}] = pack4 [get8 ini (4 * i{2}); get8 ini (4 * i{2} + 1);
-                                get8 ini (4 * i{2} + 2); get8 ini (4 * i{2} + 3)].
-    + have <- := W4u8.unpack8K k{2}.[i{2}].
-      congr; apply W4u8.Pack.all_eq_eq.
-      rewrite /all_eq /get8 /ini /init32 /= !WArray64.initiE 1..4:/# /=.
-      by rewrite mulzC !modzMDl /= modzMl mulzK 1:// !divzMDl. 
-    by rewrite /= store4u8.    
-  wp;skip => /> &2 ^ h0;rewrite W32.uleE /= => /> h1 h2 h3 h4 i ??. 
-  rewrite W32.to_uintB 1:// /=.
-  by rewrite W64.to_uintD_small 1:/# W64.to_uintD_small 1:/# /= /#. 
-qed.
-
-equiv store len0 : ChaCha20_pref.M.store ~ ChaCha20_sref.M.store :
-  ={Glob.mem} /\ output{1} = s_output{2} /\ plain{1} = s_plain{2} /\ len{1} = s_len{2} /\
-  W32.of_int 64 \ule len{1} /\ (inv_ptr output plain (to_uint len)){1} /\ len{1} = len0 /\
-  k{1} = k{2}.[15 <- k15{2}] 
-  ==>
-  ={Glob.mem, res} /\ (inv_ptr res.`1 res.`2 (to_uint res.`3)){1} /\ res{2}.`3 = len0 - W32.of_int 64.
-proof.
-  transitivity ChaCha20_pref.M.store32
-    (={Glob.mem, k, output, plain, len} /\ W32.of_int 64 \ule len{1} /\
-     (inv_ptr output plain (to_uint len)){1} /\ len{1} = len0
-     ==>
-     ={Glob.mem, res} /\ (inv_ptr res.`1 res.`2 (to_uint res.`3)){1} /\ res{1}.`3 = len0 - W32.of_int 64)
-    (={Glob.mem} /\ output{1} = s_output{2} /\ plain{1} = s_plain{2} /\ len{1} = s_len{2} /\ k{1} = k{2}.[15 <- k15{2}]
-     ==> 
-     ={Glob.mem, res}).
-  + move=> /> *; by exists Glob.mem{2} (s_output, s_plain, s_len, k.[15 <- k15]){2}.
-  + by move=> />.
-  + by apply (store_store32 len0).
-  proc => /=.  
-  sim.
-  seq 0 3 : (#pre /\ (s_k.[0] = k.[12] /\ s_k.[1] = k.[13] /\ s_k.[2] = k.[14]){2}).
-  + by unroll for{2} 3; wp;skip => />.
-  sp 0 3.
-  splitwhile {1} 2 : (i < 12).
-  seq 2 2: (={Glob.mem, output, plain, len} /\ k{1}.[12] = s_k{2}.[0] /\ 
-             k{1}.[13] = s_k{2}.[1] /\ k{1}.[14] = s_k{2}.[2] /\ k{1}.[15] = k15{2} /\ i{1} = 12).
-  + by while (={i} /\ #{/~i{1}}post /\ (0 <= i{1} <= 12) /\ (forall j, i{1} <= j < 12 => k{1}.[j] = k{2}.[j]));
-     wp;skip; smt(Array16.get_setE).
-  rcondt{1} 1; 1:by auto. 
-  rcondt{1} 3; 1:by auto. 
-  rcondt{1} 5; 1:by auto. 
-  rcondt{1} 7; 1:by auto. 
-  rcondf{1} 9; 1:by auto. 
-  by unroll for{2} 5; unroll for{2} 2; wp;skip => /> &1 &2 -> -> ->.
-qed.
-
-equiv store_last : ChaCha20_pref.M.store ~ ChaCha20_sref.M.store_last :
-  ={Glob.mem} /\ output{1} = s_output{2} /\ plain{1} = s_plain{2} /\ len{1} = s_len{2} /\
-  (len{1} \ult W32.of_int 64) /\ k{1} = k{2}.[15 <- k15{2}] 
-  ==>
-  ={Glob.mem} /\ res{1}.`3 = W32.of_int 0.
+equiv eq_store_srefi_sref : ChaCha20_srefi.M.store ~ ChaCha20_sref.M.store :
+  ={Glob.mem} /\ output{1} = to_uint s_output{2} /\ plain{1} = to_uint s_plain{2} /\ len{1} = to_uint s_len{2} /\
+  k{1} = k{2}.[15 <- k15{2}] /\
+  (64 <= len /\ good_ptr output plain len){1} ==>
+  ={Glob.mem} /\ (good_ptr res.`1 res.`2 res.`3){1} /\
+  res{1} = (to_uint res{2}.`1, to_uint res{2}.`2, to_uint res{2}.`3).
 proof.
   proc => /=.
   inline *;wp.
-  seq 0 8 :  (={Glob.mem, output, plain, len} /\ W32.to_uint len{1} < 64 /\ k{1} = s_k{2}).
-  + conseq (_ : ={Glob.mem, output, plain, len} /\ W32.to_uint len{1} < 64 /\ Array16.all_eq k{1} s_k{2} ).
-    + by move=> |> &2 ???; apply Array16.all_eq_eq.
-    by unroll for{2} 3;wp;skip => /> &2;rewrite W32.ultE.
-  while (#pre /\ j{2} = W64.of_int i{1} /\ 0 <= i{1} <= W32.to_uint len{1}).
-  + wp;skip => /> &1 &2 ???; rewrite !W32.ultE W32.to_uint_small /= 1:/#.
-    rewrite W8.xorwC /=.
-    rewrite W64.to_uint_small //= 1:/# !W2u32.to_uint_truncateu32.
-    rewrite !W64.to_uint_small //= 1,2:/#.
-    by rewrite W32.to_uint_small //= 1:/#; smt(modz_small).
-  wp;skip => /> &2 ?.
-  case: (W32.to_uint_cmp len{2}) => /> ?? i; rewrite W32.ultE => + *. 
-  rewrite W32.to_uint_small /= 1:/# => ?.
-  by rewrite (canRL _ _ len{2} i W32.to_uintK) 1:/#.
+  splitwhile{1} ^while : (i < 12).
+  while (={i, Glob.mem} /\ (forall j, i{1} <= j <= 15 => k{1}.[j] = k{2}.[j]) /\ 12 <= i{1} /\
+          output{1} = to_uint output{2} /\ plain{1} = to_uint plain{2} /\ (64 <= len /\ good_ptr output plain len){1}).
+  + wp; skip => /> &1 &2 hj hi hlen hgo hgp hi'.
+    have heq : to_uint (W64.of_int (4 * i{2})) = 4* i{2} by rewrite W64.to_uint_small /= /#.
+    have heq1 : to_uint (output{2} + W64.of_int (4 * i{2})) = to_uint output{2} + 4 * i{2}.
+    + by rewrite W64.to_uintD_small heq // /#. 
+    have heq2 : to_uint (plain{2} + W64.of_int (4 * i{2})) = to_uint plain{2} + 4 * i{2}.
+    + by rewrite W64.to_uintD_small heq // /#. 
+    smt(Array16.get_setE).
+  wp.
+  while{2} (0 <= i <= 3 /\ forall j, 0 <= j < i => k.[12 + j] = s_k.[j]){2} (3 - i{2}).
+  + move=> _ z; wp; skip => />; smt(Array16.get_setE).
+  wp.
+  while (={Glob.mem, i} /\ 0 <= i{1} <= 12 /\ (forall j, i{1} <= j < 15 => k{1}.[j] = k{2}.[j]) /\
+         output{1} = to_uint output{2} /\ plain{1} = to_uint plain{2} /\ (64 <= len /\ good_ptr output plain len){1}).
+  + wp; skip => /> &1 &2 ? hj 4?. 
+    have heq : to_uint (W64.of_int (4 * i{2})) = 4* i{2} by rewrite W64.to_uint_small /= /#.
+    have heq1 : to_uint (output{2} + W64.of_int (4 * i{2})) = to_uint output{2} + 4 * i{2}.
+    + by rewrite W64.to_uintD_small heq // /#. 
+    have heq2 : to_uint (plain{2} + W64.of_int (4 * i{2})) = to_uint plain{2} + 4 * i{2}.
+    + by rewrite W64.to_uintD_small heq // /#. 
+    smt(Array16.get_setE).
+  wp.
+  while{2}(0 <= i <= 3 /\ forall j, 0 <= j < i => k.[12 + j] = s_k.[j]){2} (3 - i{2}).
+  + move=> _ z; wp; skip => /> *; smt(Array3.get_setE).
+  wp; skip => /> *.
+  have heq1 : to_uint (s_output{2} + W64.of_int 64) = to_uint s_output{2} + 64.
+  + by rewrite W64.to_uintD_small // /#. 
+  have heq2 : to_uint (s_plain{2} + W64.of_int 64) = to_uint s_plain{2} + 64.
+  + by rewrite W64.to_uintD_small // /#.
+  have heq3 : to_uint (s_len{2} - W32.of_int 64) = to_uint s_len{2} - 64.
+  + by rewrite W32.to_uintB // uleE. 
+  rewrite heq1 heq2 heq3 /=; smt(Array16.get_setE).
 qed.
 
-equiv increment_counter: ChaCha20_pref.M.increment_counter ~ ChaCha20_sref.M.increment_counter :
+equiv eq_store_last_srefi_sref : ChaCha20_srefi.M.store_last ~ ChaCha20_sref.M.store_last :
+  ={Glob.mem} /\ output{1} = to_uint s_output{2} /\ plain{1} = to_uint s_plain{2} /\ len{1} = to_uint s_len{2} /\
+  k{1} = k{2}.[15 <- k15{2}] /\
+  (len < 64 /\ good_ptr output plain len){1} ==>
+  ={Glob.mem}.
+proof.
+  proc => /=.
+  while (={Glob.mem} /\ k{1} = s_k{2} /\ len{1} < 64 /\
+         j{1} = to_uint j{2} /\ output{1} = to_uint output{2} /\ plain{1} = to_uint plain{2} /\ len{1} = to_uint len{2} /\
+         (good_ptr output plain len){1}).
+  + wp; skip => /> &2 ???; rewrite !ultE => ?. 
+    rewrite !W2u32.to_uint_truncateu32.
+    have heq1 : to_uint (output{2} +  j{2}) = to_uint output{2} + to_uint j{2}.
+    + by rewrite W64.to_uintD_small // /#. 
+    have heq2 : to_uint (plain{2} +  j{2}) = to_uint plain{2} + to_uint j{2}.
+    + by rewrite W64.to_uintD_small // /#. 
+    have heq3 : to_uint (j{2} + W64.one) = to_uint j{2} + 1.
+    + rewrite W64.to_uintD_small //= /#.
+    rewrite heq1 heq2 heq3 /= !modz_small; smt(W64.to_uint_cmp).
+  wp.
+  while{2} (0 <= i <= 15 /\ forall j, 0 <= j < i => s_k.[j] = k.[j]){2} (15-i{2}).
+  + move=> ? z;wp; skip; smt(Array16.get_setE).    
+  wp; skip => /> &2 ???.
+  rewrite ultE /= W2u32.to_uint_truncateu32 /(%%) /=; split; 1: smt().
+  move=> i1 ?; split;1 : smt().
+  move=> ????.
+  have ->> : i1 = 15 by smt().
+  apply Array16.ext_eq=> j; rewrite !Array16.get_setE // /#.
+qed.
+
+equiv eq_increment_counter_srefi_sref: ChaCha20_srefi.M.increment_counter ~ ChaCha20_sref.M.increment_counter :
   ={st} ==> ={res}.
 proof.
   by proc;auto => /> &2;rewrite W32.WRingA.addrC.
 qed.
 
-equiv pref_sref : ChaCha20_pref.M.chacha20_ref ~ ChaCha20_sref.M.chacha20_ref : 
-  ={output, plain, len, key, nonce,counter, Glob.mem} /\
-  (inv_ptr output plain (to_uint len)){1}
+equiv eq_chacha20_srefi_sref : ChaCha20_srefi.M.chacha20_ref ~ ChaCha20_sref.M.chacha20_ref : 
+  key{1} = to_uint key{2} /\ nonce{1} = to_uint nonce{2} /\  (key + 32 < W64.modulus /\ nonce + 12 < W64.modulus){1} /\
+  output{1} = to_uint output{2} /\ plain{1} = to_uint plain{2} /\ len{1} = to_uint len{2} /\
+  (good_ptr output plain len){1} /\
+  ={Glob.mem, counter} 
   ==>
   ={Glob.mem}.
 proof.
 proc => /=.
 sp; seq 1 1 : (#{/~(_ = witness)}pre /\ ={st}).
-+ by call init;skip => />.
-splitwhile{1} 1 : (W32.of_int 64 \ule len).
++ by call eq_init_srefi_sref;skip => />.
 seq 1 1 : (={st, Glob.mem} /\ 
-           output{1} = s_output{2} /\ plain{1} = s_plain{2} /\ len{1} = s_len{2} /\
-           len{1} \ult W32.of_int 64). 
-+ while (={st, Glob.mem} /\ 
-          output{1} = s_output{2} /\ plain{1} = s_plain{2} /\ len{1} = s_len{2} /\
-          (inv_ptr output plain (to_uint len)){1}). 
-  + call increment_counter;ecall (store len{1}); call sum_states; call rounds; call copy_state.
-    skip => /> &m; rewrite W32.ultE W32.uleE /= => ????????? ->.
-    by rewrite W32.uleE W32.ultE /= W32.to_uintB 1:W32.uleE //= /#.
-  skip => /> &m;rewrite W32.uleE W32.ultE /= => *;split => [/# | s_len_R out pla].
-  by rewrite !W32.uleE !W32.ultE /= /#.
-unroll{1} 1.
-seq 1 1 : (={Glob.mem} /\ len{1} = W32.of_int 0);last first.
-+ by rcondf{1} 1; move=> *;skip => />.
-if => //;last first.
-+ skip => /> &m;rewrite !W32.ultE /= => ??.
-  apply W32.to_uintRL => /=;rewrite modz_small 1://; smt (W32.to_uint_cmp).
-inline{1}ChaCha20_pref.M.increment_counter;wp.
-call store_last; call sum_states; call rounds; call copy_state;skip => />.
+           output{1} = to_uint s_output{2} /\ plain{1} = to_uint s_plain{2} /\ len{1} = to_uint s_len{2} /\
+           (good_ptr output plain len){1} /\
+           len{1} < 64). 
++ while (#{/~ len{1} < _}post).
+  + call eq_increment_counter_srefi_sref.
+    call eq_store_srefi_sref.
+    call eq_sum_states_srefi_sref.
+    call eq_rounds_srefi_sref.
+    by ecall{2} (copy_state_sref_spec st{2});skip => /> *; rewrite uleE.
+  skip => /> *; rewrite uleE /= => ??; rewrite uleE => /#.
+if=> //.
++ by move=> /> *;rewrite ultE.
+call eq_store_last_srefi_sref.
+call eq_sum_states_srefi_sref.
+call eq_rounds_srefi_sref.
+by ecall{2} (copy_state_sref_spec st{2});skip.
 qed.
 
 
-hoare chacha20_sref_spec output0 plain0 key0 nonce0 counter0 : ChaCha20_sref.M.chacha20_ref :
-  output = output0 /\ 
-  inv_ptr output plain (to_uint len) /\
-  plain0 = loads_8 Glob.mem plain (W32.to_uint len) /\
-  key0 = Array8.of_list W32.zero (loads_32 Glob.mem key 8) /\
-  nonce0 = Array3.of_list W32.zero (loads_32 Glob.mem nonce 3) /\
-  counter0 = counter 
+hoare chacha20_sref_spec mem0 output0 plain0 key0 len0 nonce0 counter0 : ChaCha20_sref.M.chacha20_ref :
+  mem0 = Glob.mem /\ output0 = to_uint output /\ len0 = to_uint len /\
+  plain0 = loads_8 Glob.mem (to_uint plain) (to_uint len) /\
+  key0 = Array8.of_list W32.zero (loads_32 Glob.mem (to_uint key) 8) /\
+  nonce0 = Array3.of_list W32.zero (loads_32 Glob.mem (to_uint nonce) 3) /\
+  counter0 = counter /\
+  inv_ptr (to_uint output) (to_uint plain) (to_uint len) /\
+  to_uint key + 32 < W64.modulus /\ 
+  to_uint nonce + 12 < W64.modulus /\
+  to_uint output + to_uint len < W64.modulus /\ 
+  to_uint plain + to_uint len < W64.modulus 
   ==> 
   (chacha20_CTR_encrypt_bytes key0 nonce0 counter0 plain0).`1 = 
-  loads_8 Glob.mem output0 (size plain0).
+     loads_8 Glob.mem output0 len0 /\
+  mem_eq_except (in_range output0 len0) Glob.mem mem0.
 proof.
- bypr.
- move=> &m [#] ? hinv ????.
- have <-: 
-  Pr[ChaCha20_pref.M.chacha20_ref(output{m}, plain{m}, len{m}, key{m}, nonce{m}, counter{m}) @ &m :
-      (chacha20_CTR_encrypt_bytes key0 nonce0 counter0 plain0).`1 <> loads_8 Glob.mem output0 (size plain0)] =
-  Pr[ChaCha20_sref.M.chacha20_ref(output{m}, plain{m}, len{m}, key{m}, nonce{m}, counter{m}) @ &m :
-      (chacha20_CTR_encrypt_bytes key0 nonce0 counter0 plain0).`1 <> loads_8 Glob.mem output0 (size plain0)].
- + byequiv pref_sref => //=.
- byphoare (_ : output = output0 /\ 
-  inv_ptr output plain (to_uint len) /\
-  plain0 = loads_8 Glob.mem plain (W32.to_uint len) /\
-  key0 = Array8.of_list W32.zero (loads_32 Glob.mem key 8) /\
-  nonce0 = Array3.of_list W32.zero (loads_32 Glob.mem nonce 3) /\
-  counter0 = counter 
-  ==> 
-  (chacha20_CTR_encrypt_bytes key0 nonce0 counter0 plain0).`1 <> 
-  loads_8 Glob.mem output0 (size plain0)) => //.
- hoare.
- conseq (chacha20_ref_spec output0 plain0 key0 nonce0 counter0).
+  bypr.
+  move=> &m [#] h1 h2 h3 h4 h5 h6 h7 h8 h9 h10 h11 h12. 
+  have <-: 
+   Pr[ChaCha20_srefi.M.chacha20_ref(output0, to_uint plain{m}, len0, to_uint key{m}, 
+                                   to_uint nonce{m}, counter{m}) @ &m :
+       !((chacha20_CTR_encrypt_bytes key0 nonce0 counter0 plain0).`1 =loads_8 Glob.mem output0 len0 /\
+        mem_eq_on (predC (in_range output0 len0)) Glob.mem mem0)] =
+   Pr[ChaCha20_sref.M.chacha20_ref(output{m}, plain{m}, len{m}, key{m}, nonce{m}, counter{m}) @ &m :
+       !((chacha20_CTR_encrypt_bytes key0 nonce0 counter0 plain0).`1 = loads_8 Glob.mem output0 len0 /\
+          mem_eq_on (predC (in_range output0 len0)) Glob.mem mem0)].
+  + by byequiv eq_chacha20_srefi_sref => />; rewrite h2 h3.
+  have <-: 
+   Pr[ChaCha20_pref.M.chacha20_ref(output0, to_uint plain{m}, len0, to_uint key{m}, 
+                                   to_uint nonce{m}, counter{m}) @ &m :
+       !((chacha20_CTR_encrypt_bytes key0 nonce0 counter0 plain0).`1 =loads_8 Glob.mem output0 len0 /\
+        mem_eq_on (predC (in_range output0 len0)) Glob.mem mem0)] =
+   Pr[ChaCha20_srefi.M.chacha20_ref(output0, to_uint plain{m}, len0, to_uint key{m}, 
+                                    to_uint nonce{m}, counter{m}) @ &m :
+       !((chacha20_CTR_encrypt_bytes key0 nonce0 counter0 plain0).`1 = loads_8 Glob.mem output0 len0 /\
+          mem_eq_on (predC (in_range output0 len0)) Glob.mem mem0)].
+  + by byequiv eq_chacha20_pref_srefi => />; rewrite h2 h3.
+  pose plain1 := to_uint plain{m}; 
+  pose key1 := to_uint key{m};
+  pose nonce1 := to_uint nonce{m}.
+  byphoare (_: mem0 = Glob.mem /\
+   0 <= len /\
+   output = output0 /\ plain = plain1 /\ len = len0 /\ key = key1 /\ nonce = nonce1 /\
+   inv_ptr output0 plain1 len0 /\
+   plain0 = loads_8 mem0 plain1 len0 /\
+   key0 = Array8.of_list W32.zero (loads_32 mem0 key1 8) /\
+   nonce0 = Array3.of_list W32.zero (loads_32 mem0 nonce1 3) /\
+   counter0 = counter 
+   ==> 
+   !((chacha20_CTR_encrypt_bytes key0 nonce0 counter0 plain0).`1 = loads_8 Glob.mem output0 len0 /\
+     mem_eq_except (in_range output0 len0) Glob.mem mem0)) => //; last first.
+  + move=> />; rewrite h1 h2 h3 h4 /plain1 /key1 /nonce1 h8 h5 h6 /=;
+     case: (W32.to_uint_cmp len{m}) => -> //.
+  hoare => //.
+  conseq (chacha20_ref_spec mem0 output0 plain0 key0 nonce0 counter0) => //.
+  move: h1 h2 h3 h4 h5 h6 h7; rewrite /plain1 /key1 /nonce1 => /> &hr 7? mem1.
+  rewrite size_loads_8 max_ler => />; case: (W32.to_uint_cmp len{m}) => -> //.
 qed.
+
+
